end of day 21/10/19

inference-tool/src/main/java/com/lagodiuk/gp/symbolic/SymbolicRegressionEngine.java
@@ -1,0 +1,147 @@
+/*******************************************************************************
+ * Copyright 2012 Yuriy Lagodiuk
+ * Modified by Michael Foster
+ * 
+ * Licensed under the Apache License, Version 2.0 (the "License");
+ * you may not use this file except in compliance with the License.
+ * You may obtain a copy of the License at
+ * 
+ *   http://www.apache.org/licenses/LICENSE-2.0
+ * 
+ * Unless required by applicable law or agreed to in writing, software
+ * distributed under the License is distributed on an "AS IS" BASIS,
+ * WITHOUT WARRANTIES OR CONDITIONS OF ANY KIND, either express or implied.
+ * See the License for the specific language governing permissions and
+ * limitations under the License.
+ ******************************************************************************/
+package com.lagodiuk.gp.symbolic;
+
+import java.util.Collection;
+import java.util.List;
+
+import com.lagodiuk.ga.GeneticAlgorithm;
+import com.lagodiuk.ga.Fitness;
+import com.lagodiuk.ga.IterartionListener;
+import com.lagodiuk.ga.Population;
+import com.lagodiuk.gp.symbolic.interpreter.Context;
+import com.lagodiuk.gp.symbolic.interpreter.Expression;
+import com.lagodiuk.gp.symbolic.interpreter.Function;
+import com.lagodiuk.gp.symbolic.interpreter.SyntaxTreeUtils;
+
+public class SymbolicRegressionEngine {
+
+	private static final int INITIAL_PARENT_CHROMOSOMES_SURVIVE_COUNT = 1;
+
+	private static final int DEFAULT_POPULATION_SIZE = 10;
+
+	private static final int MAX_INITIAL_TREE_DEPTH = 4;
+
+	private GeneticAlgorithm<GpChromosome, Double> environment;
+
+	private Context context;
+
+	private ExpressionFitness expressionFitness;
+	
+	private Population<GpChromosome> createPopulation(
+			Context context,
+			Fitness<GpChromosome, Double> fitnessFunction,
+			int populationSize
+			) {
+		Population<GpChromosome> population = new Population<GpChromosome>();
+		for (int i = 0; i < populationSize; i++) {
+			GpChromosome chromosome = new GpChromosome(context, fitnessFunction,
+					SyntaxTreeUtils.createTree(MAX_INITIAL_TREE_DEPTH, context));
+			population.addChromosome(chromosome);
+		}
+		return population;
+	}
+
+	public SymbolicRegressionEngine(
+			int[] values,
+			ExpressionFitness expressionFitness,
+			Collection<String> variables,
+			List<? extends Function> baseFunctions
+			) {
+		this.context = new Context(values, baseFunctions, variables);
+		this.expressionFitness = expressionFitness;
+		Fitness<GpChromosome, Double> fitnessFunction = new SymbolicRegressionFitness(this.expressionFitness);
+		Population<GpChromosome> population = this.createPopulation(this.context, fitnessFunction,
+				DEFAULT_POPULATION_SIZE);
+		this.environment = new GeneticAlgorithm<GpChromosome, Double>(population, fitnessFunction);
+		this.environment.setParentChromosomesSurviveCount(INITIAL_PARENT_CHROMOSOMES_SURVIVE_COUNT);
+	}
+	
+	public SymbolicRegressionEngine(
+			List<Integer> values,
+			ExpressionFitness expressionFitness,
+			Collection<String> variables,
+			List<? extends Function> baseFunctions
+			) {
+		this.context = new Context(values, baseFunctions, variables);
+		this.expressionFitness = expressionFitness;
+		Fitness<GpChromosome, Double> fitnessFunction = new SymbolicRegressionFitness(this.expressionFitness);
+		Population<GpChromosome> population = this.createPopulation(this.context, fitnessFunction,
+				DEFAULT_POPULATION_SIZE);
+		this.environment = new GeneticAlgorithm<GpChromosome, Double>(population, fitnessFunction);
+		this.environment.setParentChromosomesSurviveCount(INITIAL_PARENT_CHROMOSOMES_SURVIVE_COUNT);
+	}
+	
+	public SymbolicRegressionEngine(
+			int[] values,
+			ExpressionFitness expressionFitness,
+			Collection<String> variables,
+			List<? extends Function> baseFunctions,
+			Expression[] extras
+			) {
+		this.context = new Context(values, baseFunctions, variables);
+		System.out.println(this.context);
+		this.expressionFitness = expressionFitness;
+		Fitness<GpChromosome, Double> fitnessFunction = new SymbolicRegressionFitness(this.expressionFitness);
+		Population<GpChromosome> population = this.createPopulation(this.context, fitnessFunction, DEFAULT_POPULATION_SIZE);
+//		Population<GpChromosome> population = new Population<GpChromosome>();
+		for (Expression e: extras) {
+			GpChromosome chromosome = new GpChromosome(context, fitnessFunction,e);
+			population.addChromosome(chromosome);
+		}
+		this.environment = new GeneticAlgorithm<GpChromosome, Double>(population, fitnessFunction);
+		this.environment.setParentChromosomesSurviveCount(INITIAL_PARENT_CHROMOSOMES_SURVIVE_COUNT);
+	}
+	
+	public void addIterationListener(final SymbolicRegressionIterationListener listener) {
+		this.environment.addIterationListener(new IterartionListener<GpChromosome, Double>() {
+			@Override
+			public void update(GeneticAlgorithm<GpChromosome, Double> environment) {
+				listener.update(SymbolicRegressionEngine.this);
+			}
+		});
+	}
+
+	public void evolve(int itrationsCount) {
+		this.environment.evolve(itrationsCount);
+	}
+
+	public Context getContext() {
+		return this.context;
+	}
+
+	public Expression getBestSyntaxTree() {
+		return this.environment.getBest().getSyntaxTree();
+	}
+
+	public double fitness(Expression expression) {
+		return this.expressionFitness.fitness(expression, this.context);
+	}
+
+	public void terminate() {
+		this.environment.terminate();
+	}
+
+	public int getIteration() {
+		return this.environment.getIteration();
+	}
+
+	public void setParentsSurviveCount(int n) {
+		this.environment.setParentChromosomesSurviveCount(n);
+	}
+
+}
