inference-tool/src/main/java/com/lagodiuk/gp/symbolic/SymbolicRegressionFitness.java
@@ -1,0 +1,37 @@
+/*******************************************************************************
+ * Copyright 2012 Yuriy Lagodiuk
+ * 
+ * Licensed under the Apache License, Version 2.0 (the "License");
+ * you may not use this file except in compliance with the License.
+ * You may obtain a copy of the License at
+ * 
+ *   http://www.apache.org/licenses/LICENSE-2.0
+ * 
+ * Unless required by applicable law or agreed to in writing, software
+ * distributed under the License is distributed on an "AS IS" BASIS,
+ * WITHOUT WARRANTIES OR CONDITIONS OF ANY KIND, either express or implied.
+ * See the License for the specific language governing permissions and
+ * limitations under the License.
+ ******************************************************************************/
+package com.lagodiuk.gp.symbolic;
+
+import com.lagodiuk.ga.Fitness;
+import com.lagodiuk.gp.symbolic.interpreter.Context;
+import com.lagodiuk.gp.symbolic.interpreter.Expression;
+
+class SymbolicRegressionFitness implements Fitness<GpChromosome, Double> {
+
+	private ExpressionFitness expressionFitness;
+
+	public SymbolicRegressionFitness(ExpressionFitness expressionFitness) {
+		this.expressionFitness = expressionFitness;
+	}
+
+	@Override
+	public Double calculate(GpChromosome chromosome) {
+		Expression expression = chromosome.getSyntaxTree();
+		Context context = chromosome.getContext();
+		return this.expressionFitness.fitness(expression, context);
+	}
+
+}
