inference-tool/src/main/java/com/lagodiuk/gp/symbolic/TabulatedFunctionFitness.java
@@ -1,0 +1,120 @@
+/*******************************************************************************
+ * Copyright 2012 Yuriy Lagodiuk
+ * Modified by Michael Foster
+ * 
+ * Licensed under the Apache License, Version 2.0 (the "License");
+ * you may not use this file except in compliance with the License.
+ * You may obtain a copy of the License at
+ * 
+ *   http://www.apache.org/licenses/LICENSE-2.0
+ * 
+ * Unless required by applicable law or agreed to in writing, software
+ * distributed under the License is distributed on an "AS IS" BASIS,
+ * WITHOUT WARRANTIES OR CONDITIONS OF ANY KIND, either express or implied.
+ * See the License for the specific language governing permissions and
+ * limitations under the License.
+ ******************************************************************************/
+package com.lagodiuk.gp.symbolic;
+
+import java.util.HashSet;
+import java.util.LinkedList;
+import java.util.List;
+import java.util.Set;
+
+import com.lagodiuk.gp.symbolic.interpreter.Context;
+import com.lagodiuk.gp.symbolic.interpreter.Expression;
+
+public class TabulatedFunctionFitness implements ExpressionFitness {
+
+	private List<Target> targets = new LinkedList<Target>();
+
+	public TabulatedFunctionFitness(Target... targets) {
+		for (Target target : targets) {
+			this.targets.add(target);
+		}
+	}
+
+	public TabulatedFunctionFitness(List<Target> targets) {
+		this.targets.addAll(targets);
+	}
+	
+	public List<Target> getTargets() {
+		return this.targets;
+	}
+	
+	@Override
+	public double fitness(Expression expression, Context context) {
+		double diff = 0.0;
+		double mistakes = 0.0;
+		Set<String> totalUsedVars = new HashSet<String>();
+		
+		for (Target target : this.targets) {
+			Set<String> usedVars = target.getContextState().keySet();
+			for (String v: usedVars) {
+				totalUsedVars.add(v);
+			}
+			
+			double targetValue = target.getTargetValue();
+			
+			Set<String> undef = context.dom();
+			undef.removeAll(usedVars);
+			context.setup(target.getContextState().entrySet());
+
+			double minErr = Double.POSITIVE_INFINITY;
+			
+			if (undef.isEmpty()) {
+				double offBy = Math.abs(targetValue - expression.eval(context));
+				if (offBy < minErr) {
+					minErr = offBy;
+				}
+			}
+			else {
+				for (String v: undef) {
+					for (int i: context.getValues()) {
+						context.setVariable(v, i);
+						double offBy = Math.abs(targetValue - expression.eval(context));
+						if (offBy < minErr) {
+							minErr = offBy;
+						}
+					}
+				}
+			}
+			
+			diff += minErr;
+			if (minErr > 0) {
+				mistakes++;
+			}
+		}
+		
+		totalUsedVars.removeAll(expression.vars());
+		
+		return mistakes + (diff/this.targets.size()) + totalUsedVars.size() + expression.vars().size();
+	}
+	
+//	This is solidly OK most of the time.
+//	public double fitness(Expression expression, Context context) {
+//		int diff = 0;
+//		int mistakes = 0;
+//		
+//		for (Target target : this.targets) {
+//			Set<String> undef = context.dom();
+//			undef.removeAll(target.getContextState().keySet());
+//			
+//			for (String v: undef) {
+//				context.setVariable(v, context.getRandomValue());
+//			}
+//			context.setup(target.getContextState().entrySet());
+//			
+//			int targetValue = target.getTargetValue();
+//			int calculatedValue = expression.eval(context);
+//			double offBy = Math.abs(targetValue - calculatedValue);
+//			diff += offBy/(offBy+1);
+//			if (targetValue != calculatedValue) {
+//				mistakes++;
+//			}
+//		}
+//		
+//		return mistakes + (diff/this.targets.size());
+//	}
+	
+}
