inference-tool/src/main/java/com/lagodiuk/gp/symbolic/Target.java
@@ -1,0 +1,121 @@
+/*******************************************************************************
+ * Copyright 2012 Yuriy Lagodiuk
+ * Modified by Michael Foster
+ * 
+ * Licensed under the Apache License, Version 2.0 (the "License");
+ * you may not use this file except in compliance with the License.
+ * You may obtain a copy of the License at
+ * 
+ *   http://www.apache.org/licenses/LICENSE-2.0
+ * 
+ * Unless required by applicable law or agreed to in writing, software
+ * distributed under the License is distributed on an "AS IS" BASIS,
+ * WITHOUT WARRANTIES OR CONDITIONS OF ANY KIND, either express or implied.
+ * See the License for the specific language governing permissions and
+ * limitations under the License.
+ ******************************************************************************/
+package com.lagodiuk.gp.symbolic;
+
+import java.util.ArrayList;
+import java.util.Collections;
+import java.util.HashMap;
+import java.util.List;
+import java.util.Map;
+import java.util.Set;
+
+import com.lagodiuk.gp.symbolic.interpreter.Expression;
+import com.microsoft.z3.Context;
+import com.microsoft.z3.FuncDecl;
+import com.microsoft.z3.Model;
+import com.microsoft.z3.Solver;
+
+public class Target {
+	private Map<String, Integer> contextState = new HashMap<String, Integer>();
+	private int targetValue;
+
+	public Target() {
+	}
+
+	public Target(Map<String, Integer> contextState, int targetValue) {
+		this.contextState.putAll(contextState);
+		this.targetValue = targetValue;
+	}
+	
+	public Target(int targetValue, Integer... inputs) {
+		int i = 1;
+		for (int iv: inputs) {
+			this.when("i"+i, iv);
+		}
+		this.targetValue = targetValue;
+	}
+
+	public Target when(String variableName, int variableValue) {
+		this.contextState.put(variableName, variableValue);
+		return this;
+	}
+
+	public Target targetIs(int targetValue) {
+		this.targetValue = targetValue;
+		return this;
+	}
+
+	public int getTargetValue() {
+		return this.targetValue;
+	}
+
+	public Map<String, Integer> getContextState() {
+		return this.contextState;
+	}
+	
+	public void solve(Expression expression) {
+		List<String> expVars = new ArrayList<>(expression.vars());
+		Collections.sort(expVars);
+
+		Set<String> definedVars = this.getContextState().keySet();
+		
+		List<String> undefinedVars = new ArrayList<>(expVars);
+		undefinedVars.removeAll(definedVars);
+		
+		String inputs = "";
+		for (String v : expVars) {
+			inputs += "("+v +" Int)";
+		}
+
+		String z3String = "(define-fun f ("+inputs+") Int \n  "+expression+"\n)\n";
+		
+		for (String v: undefinedVars) {
+			z3String += "(declare-const "+v+" Int)\n";
+		}
+		
+		List<String> args = new ArrayList<String>();
+		
+		for (String v: expVars) {
+			if (definedVars.contains(v)) {
+				args.add(this.getContextState().get(v).toString());
+			}
+			else {
+				args.add(v);
+			}
+		}
+		
+		String assertion = "(assert (= "+this.getTargetValue()+" (f "+String.join(" ", args)+")))";
+
+		z3String += assertion;
+		
+//		System.out.println(z3String);
+		
+        Context ctx = new Context();
+        Solver solver = ctx.mkSimpleSolver();
+        solver.fromString(z3String);
+        solver.check();
+        Model model = solver.getModel();
+        for (FuncDecl f: model.getConstDecls()) {
+        	this.when(f.getName().toString(), Integer.valueOf(model.getConstInterp(f).toString()));
+        }
+        ctx.close();
+	}
+	
+	public String toString() {
+		return this.getContextState().entrySet() + " -> " + this.targetValue;
+	}
+}
