inference-tool/src/main/java/com/lagodiuk/gp/symbolic/interpreter/Expression.java
@@ -1,0 +1,264 @@
+/*******************************************************************************
+ * Copyright 2012 Yuriy Lagodiuk
+ * Modified by Michael Foster
+ *
+ * Licensed under the Apache License, Version 2.0 (the "License");
+ * you may not use this file except in compliance with the License.
+ * You may obtain a copy of the License at
+ *
+ *   http://www.apache.org/licenses/LICENSE-2.0
+ *
+ * Unless required by applicable law or agreed to in writing, software
+ * distributed under the License is distributed on an "AS IS" BASIS,
+ * WITHOUT WARRANTIES OR CONDITIONS OF ANY KIND, either express or implied.
+ * See the License for the specific language governing permissions and
+ * limitations under the License.
+ ******************************************************************************/
+package com.lagodiuk.gp.symbolic.interpreter;
+
+import java.util.ArrayList;
+import java.util.Arrays;
+import java.util.Collections;
+import java.util.Deque;
+import java.util.LinkedList;
+import java.util.List;
+import java.util.Set;
+
+import com.microsoft.z3.ArithExpr;
+import com.microsoft.z3.Context;
+import com.microsoft.z3.Expr;
+
+public class Expression implements Cloneable {
+
+	private List<Expression> childs = new ArrayList<Expression>();
+
+	private List<Integer> coefficients = new ArrayList<Integer>();
+
+	private String variable;
+
+	private Function function;
+
+	public Expression(Function function) {
+		this.function = function;
+	}
+
+	public int eval(com.lagodiuk.gp.symbolic.interpreter.Context context) {
+		return this.function.eval(this, context);
+	}
+
+	public Set<String> vars() {
+		return this.function.vars(this);
+	}
+
+	public int height() {
+		return this.function.height(this);
+	}
+
+	public String print() {
+		return this.function.print(this);
+	}
+
+	public List<Expression> getChilds() {
+		return this.childs;
+	}
+
+	public Expression setChilds(List<Expression> childs) {
+		this.childs = childs;
+		return this;
+	}
+
+	public void addChild(Expression child) {
+		this.childs.add(child);
+	}
+
+	public void removeChilds() {
+		this.childs.clear();
+	}
+
+	public List<Integer> getCoefficientsOfNode() {
+		return this.coefficients;
+	}
+
+	public Expression setCoefficientsOfNode(List<Integer> coefficients) {
+		this.coefficients = coefficients;
+		return this;
+	}
+
+	public void addCoefficient(int coefficient) {
+		this.coefficients.add(coefficient);
+	}
+
+	public void removeCoefficients() {
+		if (this.coefficients.size() > 0) {
+			this.coefficients.clear();
+		}
+	}
+
+	public String getVariable() {
+		return this.variable;
+	}
+
+	public Expression setVariable(String variable) {
+		this.variable = variable;
+		return this;
+	}
+
+	public Function getFunction() {
+		return this.function;
+	}
+
+	public void setFunction(Function function) {
+		this.function = function;
+	}
+
+	@Override
+	public Expression clone() {
+		Expression cloned = new Expression(this.function);
+		if (this.variable != null) {
+			cloned.variable = new String(this.variable);
+		}
+		for (Expression c : this.childs) {
+			cloned.childs.add(c.clone());
+		}
+		for (Integer d : this.coefficients) {
+			cloned.coefficients.add(d);
+		}
+		return cloned;
+	}
+
+	public List<Integer> getCoefficientsOfTree() {
+		LinkedList<Integer> coefficients = new LinkedList<Integer>();
+		this.getCoefficientsOfTree(coefficients);
+		Collections.reverse(coefficients);
+		return coefficients;
+	}
+
+	private void getCoefficientsOfTree(Deque<Integer> coefficients) {
+		List<Integer> coeffs = this.function.getCoefficients(this);
+		for (Integer d : coeffs) {
+			coefficients.push(d);
+		}
+		for (int i = 0; i < this.childs.size(); i++) {
+			this.childs.get(i).getCoefficientsOfTree(coefficients);
+		}
+	}
+
+	public void setCoefficientsOfTree(List<Integer> coefficients) {
+		this.setCoefficientsOfTree(coefficients, 0);
+	}
+
+	private int setCoefficientsOfTree(List<Integer> coefficients, int index) {
+		this.function.setCoefficients(this, coefficients, index);
+		index += this.function.coefficientsCount();
+		if (this.childs.size() > 0) {
+			for (int i = 0; i < this.childs.size(); i++) {
+				index = this.childs.get(i).setCoefficientsOfTree(coefficients, index);
+			}
+		}
+		return index;
+	}
+
+	public List<Expression> getAllNodesAsList() {
+		List<Expression> nodes = new LinkedList<Expression>();
+		this.getAllNodesBreadthFirstSearch(nodes);
+		return nodes;
+	}
+
+	/**
+	 * non-recursive Breadth-first iteration over all node of syntax tree
+	 */
+	private void getAllNodesBreadthFirstSearch(List<Expression> nodesList) {
+		int indx = 0;
+		nodesList.add(this);
+		while (true) {
+			if (indx < nodesList.size()) {
+				Expression node = nodesList.get(indx++);
+				for (Expression child : node.childs) {
+					nodesList.add(child);
+				}
+			} else {
+				break;
+			}
+		}
+	}
+
+	public ArithExpr toZ3(Context ctx) {
+		return this.function.toZ3(this, ctx);
+	}
+
+	public Functions whatIs(Expr e) {
+		if (e.isMul()) {
+			return Functions.MUL;
+		}
+		if (e.isAdd()) {
+			return Functions.ADD;
+		}
+		if (e.isSub()) {
+			return Functions.SUB;
+		}
+		if (e.isConst()) {
+			return Functions.VARIABLE;
+		}
+		if (e.isIntNum()) {
+			return Functions.CONSTANT;
+		}
+		throw new IllegalArgumentException("Expression is not ADD, SUB, VARIABLE, or CONSTANT");
+	}
+
+	private Expression makeBinary(Expr[] e, Function f) {
+		if (e.length == 0) {
+			throw new IllegalArgumentException("Not enough args for function");
+		}
+		Expression left = fromZ3(e[0]);
+		if (e.length == 1) {
+			return left;
+		}
+		Expression expr = new Expression(f);
+		Expression right = makeBinary(Arrays.copyOfRange(e, 1, e.length), f);
+		expr.addChild(left);
+		expr.addChild(right);
+		return expr;
+	}
+
+	public Expression fromZ3(Expr ex) {
+		Functions f = whatIs(ex);
+		Expression expr = new Expression(f);
+
+		switch (f) {
+		case CONSTANT:
+			expr.addCoefficient(Integer.parseInt(ex.toString()));
+			return expr;
+		case VARIABLE:
+			expr.setVariable(ex.toString());
+			return expr;
+		case ADD:
+			return makeBinary(ex.getArgs(), Functions.ADD);
+		case MUL:
+			return makeBinary(ex.getArgs(), Functions.MUL);
+		case SUB:
+			return makeBinary(ex.getArgs(), Functions.SUB);
+		default:
+			break;
+		}
+		throw new IllegalArgumentException("Simplified expression is not ADD, SUB, VARIABLE, or CONSTANT");
+	}
+
+	public Expression simplify() {
+		Context ctx = new Context();
+		Expr ex = this.function.toZ3(this, ctx).simplify();
+		Expression simpler;
+		try {
+			simpler =  fromZ3(ex);
+		}
+		catch (NumberFormatException e) {
+			simpler = this.clone();
+		}
+		ctx.close();
+		return simpler;
+	}
+
+	public String toString() {
+		return this.print();
+	}
+
+}
