formal/inference/heuristics/Symbolic_Regression.thy
@@ -4,129 +4,105 @@ begin
 
 hide_const I
 
-datatype numOrStr = N | S
+type_synonym indexed_execution = "(nat \<times> label \<times> inputs \<times> value list) list"
+type_synonym indexed_log = "(nat \<times> indexed_execution) list"
+type_synonym flat_log = "(nat \<times> nat \<times> label \<times> inputs \<times> value list) list"
 
-fun typeChecks :: "numOrStr list \<Rightarrow> value list \<Rightarrow> bool" where
-  "typeChecks [] [] = True" |
-  "typeChecks (N#tt) ((Num _)#tv) = typeChecks tt tv" |
-  "typeChecks (S#tt) ((value.Str _)#tv) = typeChecks tt tv" |
-  "typeChecks _ _ = False"
+fun flatten :: "indexed_log \<Rightarrow> flat_log \<Rightarrow> flat_log" where
+  "flatten [] l = l" |
+  "flatten ((k, e)#t) l = flatten t (l@(map (\<lambda>v. (k, v)) e))"
 
-definition gather_events :: "log \<Rightarrow> label \<Rightarrow> numOrStr list \<Rightarrow> numOrStr list \<Rightarrow> (label \<times> value list \<times> value list) list" where
-  "gather_events ls label inputTypes outputTypes = fold List.union (
-     map
-      (\<lambda>trace. filter (\<lambda>(label', inputs, outputs). label' = label \<and> typeChecks inputTypes inputs \<and> typeChecks outputTypes outputs)
-     trace)
-   ls) []"
-
-definition is_fun :: "inputs list \<Rightarrow> inputs \<Rightarrow> nat \<Rightarrow> value list \<Rightarrow> bool" where
-  "is_fun Inputs Regs numExtraRegs Output = (\<exists>f (R :: value list list). length R = length Inputs \<and> (\<forall>r \<in> set R. length r = numExtraRegs) \<and> (\<forall>(i, r, p) \<in> set (zip Inputs (zip R Output)). f i (Regs@r) = p))"
-
-lemma "is_fun [[Num 50], [Num 100]] [] 0 [Num 50, Num 100]"
-  apply (simp add: is_fun_def)
-  apply (rule_tac x="\<lambda>i r. hd i" in exI)
-  apply (rule_tac x="[[], []]" in exI)
-  by simp
-
-lemma "\<not>is_fun [[Num 50], [Num 50]] [] 0 [Num 50, Num 100]"
-  apply (simp add: is_fun_def)
-  apply clarify
-  apply (case_tac R)
-   apply simp
-  apply (case_tac list)
-  by auto
-
-lemma "is_fun [[Num 50], [Num 50]] [] 1 [Num 50, Num 100]"
-  apply (simp add: is_fun_def)
-  apply (rule_tac x="\<lambda>i r. case (hd i, hd r) of (Num n, Num n') \<Rightarrow> Num (n+n')" in exI)
-  apply (rule_tac x="[[Num 0], [Num 50]]" in exI)
-  by simp
-
-(*
-  This gives us a minimal register assignment such that there is a deterministic function which
-  produces the correct outputs given the inputs. This will be a series of calls to Z3 in the
-  executable implementation.
-*)
-definition get_assignments :: "inputs list \<Rightarrow> inputs \<Rightarrow> value list list \<Rightarrow> inputs" where
-  "get_assignments i r P = Eps (\<lambda>R. \<forall>p \<in> set P.
-     \<comment> \<open>A function which takes these inputs and register values this many extra registers and
-         produces the correct outputs.\<close>
-    is_fun i r (length R) p \<and>
-     \<comment> \<open>Make sure it's the fewest possible additional registers\<close>
-    (\<nexists> r'. r' < length R \<and> is_fun i r r' p)
+\<comment> \<open>This will be replaced by symbolic regression in the executable\<close>
+definition get_function :: "nat \<Rightarrow> int list \<Rightarrow> inputs list \<Rightarrow> value list \<Rightarrow> aexp option" where
+  "get_function maxReg values I P = (let
+    possible_funs = {a. \<forall>(i, p) \<in> set (zip I P). \<exists>r. aval a (join_ir i r) = Some p}
+    in
+    if possible_funs = {} then None else Some (Eps (\<lambda>x. x \<in> possible_funs))
   )"
 
-(*
-  This gives us an aexp which, when evaluated with the inputs and registers, produces the correct
-  outputs. If no such aexp exists, it returns None.
-*)
-definition get_aexp :: "inputs list \<Rightarrow> inputs \<Rightarrow> value list \<Rightarrow> aexp option" where
-  "get_aexp i r p = (let
-    aexp_pred = (\<lambda>a. \<forall>(i, p) \<in> set (zip i p). aval a (join_ir i (input2state r)) = Some p) in
-    if \<exists>a. aexp_pred a then Some (Eps aexp_pred) else None
-  )"
+definition get_inputs :: "flat_log \<Rightarrow> inputs list" where
+  "get_inputs l = map (\<lambda>(_, _, _, i, _). i) l"
 
-fun type_of :: "value \<Rightarrow> numOrStr" where
-  "type_of (Num _) = N" |
-  "type_of (value.Str _) = S"
+definition get_outputs :: "flat_log \<Rightarrow> nat \<Rightarrow> value list" where
+  "get_outputs l n = map (\<lambda>(_, _, _, _, p). p ! n) l"
 
-definition exits :: "transition_matrix \<Rightarrow> transition \<Rightarrow> cfstate \<Rightarrow> bool" where
-  "exits e t s = (ffilter (\<lambda>((origin, _), t'). origin = s \<and> t' = t) e \<noteq> {||})"
+definition get_functions :: "nat \<Rightarrow> int list \<Rightarrow> nat \<Rightarrow> flat_log \<Rightarrow> aexp option list" where
+  "get_functions maxReg values n l = map (\<lambda>p. get_function maxReg values (get_inputs l) (get_outputs l p)) [0..<n]"
 
-fun walk_up_to_choice :: "transition_matrix \<Rightarrow> cfstate \<Rightarrow> registers \<Rightarrow> execution \<Rightarrow> cfstate \<Rightarrow> transition \<Rightarrow> transition \<Rightarrow> (numOrStr list \<times> numOrStr list \<times> value list) option" where
-  "walk_up_to_choice _ _ _ [] _ _ _ = None" |
-  "walk_up_to_choice e s r ((l, i, p)#t) s' t1 t2 = (
-    let possSteps = possible_steps e s r l i in
-    if s = s' \<and> l = (Label t1) \<and> exits e t1 s \<and> exits e t2 s \<and> possSteps \<noteq> {||} then
-      Some (map type_of i, map type_of p, map (\<lambda>reg. case r $ reg of Some v \<Rightarrow> v) (finfun_to_list r))
-    else
-      let
-      possibleTypes = ffilter (\<lambda>x. x \<noteq> None) (fimage (\<lambda>(dest, tr). walk_up_to_choice e dest (apply_updates (Updates tr) (join_ir i r) r) t s' t1 t2) possSteps);
-      types = fimage (\<lambda>r. case r of Some (x, y, z) \<Rightarrow> (x, y)) possibleTypes;
-      regs =  fimage (\<lambda>r. case r of Some (x, y, z) \<Rightarrow> z) possibleTypes
-      in
-      if fis_singleton types \<and> fis_singleton regs then Some (fst (fthe_elem types), snd (fthe_elem types), fthe_elem regs) else None
-  )"
+\<comment> \<open>This will be replaced to calls to Z3 in the executable\<close>
+definition get_regs :: "inputs \<Rightarrow> aexp \<Rightarrow> value \<Rightarrow> registers" where
+  "get_regs i a v = Eps (\<lambda>r. aval a (join_ir i r) = Some v)"
 
-(*
-  This gives us an aexp from a log and two transitions for a particular output
-*)
-definition symbolic_regression :: "log \<Rightarrow> transition \<Rightarrow> transition \<Rightarrow> cfstate \<Rightarrow> iEFSM \<Rightarrow> (aexp list \<times> value list) option" where
-  "symbolic_regression log t1 t2 s new = (let
-     maybe_io_types = set (map (\<lambda>p. case p of Some x \<Rightarrow> x) (filter (\<lambda>x. x \<noteq> None) (map (\<lambda>ex. walk_up_to_choice (tm new) 0 <> ex s t1 t2) log)))
-     in
-     if is_singleton maybe_io_types then let
-        (i_types, o_types, regValues) = the_elem maybe_io_types;
-        events = gather_events log (Label t1) i_types o_types;
-        inputs = map (\<lambda>(label, inputs, outputs). inputs) events;
-        (Outputs:: value list list) = map (\<lambda>(label, inputs, outputs). outputs) events;
-        registers = get_assignments inputs regValues Outputs;
-        funs = map (\<lambda>outputs. get_aexp inputs registers outputs) Outputs
-       in
-       if \<exists>p \<in> set funs. p = None then Some (map (\<lambda>p. case p of Some a \<Rightarrow> a) funs, registers) else None
-     else
-        None
+definition finfun2pairs :: "('a::linorder \<Rightarrow>f 'b) \<Rightarrow> ('a \<times> 'b) list" where
+  "finfun2pairs f = (let
+    keys = finfun_to_list f;
+    values = map (\<lambda>k. f $ k) keys
+    in zip keys values
    )"
 
-(*
-  This will be replaced by a call to Neil's thing to get us register update functions
-*)
-definition call_Neils_thing :: "iEFSM \<Rightarrow> iEFSM" where
-  "call_Neils_thing i = i"
+fun replace_transitions :: "(tid \<times> transition) list \<Rightarrow> iEFSM \<Rightarrow> iEFSM" where
+  "replace_transitions [] e = e" |
+  "replace_transitions ((ti, t)#rest) e = replace_transitions rest (fimage (\<lambda>(id', od, t'). if id' = ti then (id', od, t) else (id', od, t')) e)"
+
+fun put_output_function_aux :: "nat \<Rightarrow> aexp \<Rightarrow> indexed_execution \<Rightarrow> label \<Rightarrow> arity \<Rightarrow> arity \<Rightarrow> tid option \<Rightarrow> iEFSM \<Rightarrow> cfstate \<Rightarrow> registers \<Rightarrow> iEFSM option" where
+  "put_output_function_aux _ _ [] _ _ _ _ e _ _ = Some e" |
+  "put_output_function_aux fi f ((_, l, i, p)#t) label i_arity o_arity prevtid e s r = (
+    let
+    poss_steps = ffilter (\<lambda>(_, _, t). apply_outputs (Outputs t) (join_ir i r) = map Some p) (i_possible_steps e s r l i) in
+    \<comment> \<open>No possible steps with matching output means something bad has happenned\<close>
+    case random_member poss_steps of
+      None \<Rightarrow> None |
+      Some (tid, s', ta) \<Rightarrow>
+       \<comment> \<open>Possible steps with a transition we need to modify\<close>
+      if l = label \<and> length i \<noteq> i_arity \<and> length p \<noteq> o_arity then let
+        newT = \<lparr>Label = Label ta, Arity = Arity ta, Guard = Guard ta, Outputs = list_update (Outputs ta) fi f, Updates = Updates ta\<rparr>;
+        necessaryRegs = get_regs i f (p!fi);
+        updates = map (\<lambda>r. case (necessaryRegs $ r) of Some v' \<Rightarrow> (r, L v')) (finfun_to_list necessaryRegs) in
+        case prevtid of None \<Rightarrow> None | Some prevtid \<Rightarrow> let
+        prevT = get_by_id e prevtid;
+        newPrevT = \<lparr>Label = Label prevT, Arity = Arity prevT, Guard = Guard prevT, Outputs = Outputs prevT, Updates = (Updates prevT)@updates\<rparr>;
+        newE = replace_transitions [(tid, newT), (prevtid, newPrevT)] e
+        in
+        put_output_function_aux fi f t label i_arity o_arity (Some tid) newE s' (apply_updates (Updates ta) (join_ir i r) r)
+       \<comment> \<open>Possible steps but not interesting - just take a transition and move on\<close>
+      else
+        put_output_function_aux fi f t label i_arity o_arity (Some tid) e s' (apply_updates (Updates ta) (join_ir i r) r)
+  )"
+
+primrec put_output_function :: "nat \<Rightarrow> aexp \<Rightarrow> indexed_log \<Rightarrow> transition \<Rightarrow> iEFSM \<Rightarrow> iEFSM option" where
+  "put_output_function _ _ [] _ e = Some e" |
+  "put_output_function fi f (h#t) t1 e = (case put_output_function_aux fi f (snd h) (Label t1) (Arity t1) (length (Outputs t1)) None e 0 <> of
+    None \<Rightarrow> None |
+    Some e' \<Rightarrow> put_output_function fi f t t1 e')"
+
+fun put_output_functions :: "(nat \<times> aexp option) list \<Rightarrow> indexed_log \<Rightarrow> transition \<Rightarrow> iEFSM \<Rightarrow> iEFSM option" where
+  "put_output_functions [] _ _ e = Some e" |
+  "put_output_functions ((_, None)#_) _ _ _ = None" |
+  "put_output_functions ((fi, Some f)#rest) log t e = (case put_output_function fi f log t e of
+    None \<Rightarrow> None |
+    Some e' \<Rightarrow> put_output_functions rest log t e'
+   )"
+
+definition enumerate_value_ints :: "value list \<Rightarrow> int list" where
+  "enumerate_value_ints vs = map (\<lambda>v. case v of Num n \<Rightarrow> n) (filter (\<lambda>v. case v of Num _ \<Rightarrow> True | value.Str _ \<Rightarrow> False) vs)"
+
+definition enumerate_exec_ints :: "execution \<Rightarrow> int list" where
+  "enumerate_exec_ints vs = fold (\<lambda>(_, i, p) I. (enumerate_value_ints i) @ (enumerate_value_ints p) @ I) vs []"
+
+definition enumerate_log_ints :: "log \<Rightarrow> int list" where
+  "enumerate_log_ints l = fold (\<lambda>e I. enumerate_exec_ints e @ I) l []"
 
 fun infer_output_functions :: "log \<Rightarrow> update_modifier" where
   "infer_output_functions log t1ID t2ID s new old _ = (let
      t1 = (get_by_id new t1ID);
      t2 = (get_by_id new t2ID);
-     orig = origin t1ID new;
-     dest1 = dest t1ID new;
-     dest2 = dest t2ID new;
-     maxReg = total_max_reg new in
-     case symbolic_regression log t1 t2 s new of
-      None \<Rightarrow> None |
-      Some (op, regs) \<Rightarrow>
-        let newT = \<lparr>Label = Label t1, Arity = Arity t1, Guard = map (\<lambda>(r, v). Eq (V (R r)) (L v)) (enumerate maxReg regs) , Outputs = op, Updates = Updates t1\<rparr> in 
-        Some ((drop_transitions new {|t1ID, t2ID|}) |\<union>| {|(t1ID, (orig, dest1), newT), (t2ID, (orig, dest2), newT)|})
+     i_log = enumerate 0 (map (enumerate 0) log);
+     num_outs = length (Outputs t1);
+     relevant_events = flatten (map (\<lambda>(i, ex). (i, filter (\<lambda>(_, l, ip, op). l = Label t1 \<and> length ip = Arity t1 \<and> length op = num_outs) ex)) i_log) [];
+     values = enumerate_log_ints log;
+     max_reg = max_reg_total new;
+     output_functions = get_functions max_reg values (length (Outputs t1)) relevant_events
+     in put_output_functions (enumerate 0 output_functions) i_log t1 new
    )"
 
 end
